#todo aggiungi definizione e funzionamento

![[flip flop JK.svg]]

| J   | K   | y(t+1)            |
| --- | --- | ----------------- |
| 0   | 0   | $y(t)$            |
| 0   | 1   | 0                 |
| 1   | 0   | 1                 |
| 1   | 1   | $\overline{y(t)}$ |
#todo what the hell is this thing (**crying emoji**) :skull:
$y(t+1)=(s+y)\overline{r}=(j\overline{y}+y)(\overline{ky})=(j\overline{y}+y)(\overline{k}+y)=j\overline{y}\overline{k}+j\overline{y}\overline{y}+y\overline{l}+y\overline{y}=j\overline{y}+y\overline{k}$
